theories/progLog.v
@@ -1,152 +1,40 @@
 From iris.proofmode Require Import proofmode.
 From iris.base_logic Require Export invariants gen_heap.
-From iris.program_logic Require Export weakestpre ectx_lifting.
+From iris.program_logic Require Export weakestpre ectx_lifting total_lifting total_weakestpre.
 From iris.algebra Require Import frac auth gmap excl.
 From Coq.Lists Require Import List.
-From ASMinCoq Require Import CpdtTactics.
-
-Section wp'.
-  Context {Λ : language} `{!irisGS_gen hlc Λ Σ}.
-
-  Lemma wp_lift_atomic_step_no_fork_fupd {s E1 E2 Φ} e1 :
-    to_val e1 = None →
-    (∀ σ1 ns κ κs nt, state_interp σ1 ns (κ ++ κs) nt ={E1}=∗
-      ⌜if s is NotStuck then reducible e1 σ1 else True⌝ ∗
-      ∀ e2 σ2 efs, ⌜prim_step e1 σ1 κ e2 σ2 efs⌝ -∗ £ 1 ={E1}[E2]▷=∗
-        ⌜efs = []⌝ ∗ state_interp σ2 (S ns) κs nt ∗ from_option Φ False (to_val e2))
-    ⊢ WP e1 @ s; E1 {{ Φ }}.
-  Proof.
-    iIntros (?) "H". iApply wp_lift_atomic_step_fupd; [done|].
-    iIntros (σ1 ns κ κs nt) "Hσ1". iMod ("H" $! σ1 with "Hσ1") as "[$ H]"; iModIntro.
-    iIntros (v2 σ2 efs Hstep) "Hcred".
-    iMod ("H" $! v2 σ2 efs with "[# //] Hcred") as "H".
-    iIntros "!> !>". iMod "H" as "(-> & ? & ?) /=". by iFrame.
-  Qed.
-
-
-End wp'.
-
-
-From ASMinCoq Require Export AsmGen.
-
-
-(* CMRA for invariants *)
-Class invG Σ := InvG {
-  inv_invG : invGS Σ;}.
-
-(* CMRΑ for memory *)
-Class memG Σ := MemG {
-  mem_gen_memG :: gen_heapGS Addr Word Σ}.
-
-(* CMRA for registers *)
-Class regG Σ := RegG {
-  reg_gen_regG :: gen_heapGS Reg Word Σ; }.
-
-
-(* Stuff for the trace copied from Katamaran *)
-Class traceG (Trace : Type) Σ := TraceG {
-    trace_inG :: inG Σ (authR (optionUR (exclR (leibnizO Trace))));
-    trace_name : gname
-}.
-
-Definition tracePreΣ (Trace : Type) : gFunctors := #[GFunctor (authR (optionUR (exclR (leibnizO Trace))))].
-
-Class trace_preG (Trace : Type) Σ := {
-  trace_preG_inG :: inG Σ (authR (optionUR (exclR (leibnizO Trace))));
-}.
-
-#[export] Instance traceG_preG `{traceG T Σ} : trace_preG T Σ.
-Proof. constructor. typeclasses eauto. Defined.
-
-#[export] Instance subG_tracePreΣ {Σ T}:
-  subG (tracePreΣ T) Σ →
-  trace_preG T Σ.
-Proof. solve_inG. Qed.
-
-Section S.
-  Context `{!traceG T Σ}.
-
-  Definition tr_auth (t: T) : iProp Σ := own trace_name (● (Some (Excl (t: leibnizO T)))).
-  Definition tr_frag (t: T) : iProp Σ := own trace_name (◯ (Some (Excl (t: leibnizO T)))).
-
-  Lemma trace_full_frag_eq t t':
-    tr_auth t -∗ tr_frag t' -∗
-    ⌜ t = t' ⌝.
-  Proof.
-    iIntros "H1 H2".
-    iDestruct (own_valid_2 with "H1 H2") as %[Hi Hv]%auth_both_valid_discrete.
-    rewrite Excl_included in Hi.  apply leibniz_equiv in Hi. subst; auto.
-  Qed.
-
-  Lemma tr_frag_excl t t' :
-    tr_frag t -∗ tr_frag t' -∗ ⌜ False ⌝.
-  Proof.
-    iIntros "H1 H2". iDestruct (own_valid_2 with "H1 H2") as %Hv.
-    now apply excl_auth.excl_auth_frag_op_valid in Hv.
-  Qed.
-
-  Lemma trace_update t t' :
-    tr_auth t ∗ tr_frag t ==∗
-    tr_auth t' ∗ tr_frag t'.
-  Proof.
-    rewrite /tr_auth /tr_frag. rewrite -!own_op.
-    iApply own_update. apply auth_update.
-    apply option_local_update.
-    apply exclusive_local_update. constructor.
-  Qed.
-
-  (* For the moment, there is no need for a lemma stating that traces can only be appened to, but we could customize the RA to enforce this. *)
-
-  #[export] Instance tr_auth_Timeless t : Timeless (tr_auth t).
-  Proof.
-    intros. apply _.
-  Qed.
-
-  #[export] Instance tr_frag_Timeless t : Timeless (tr_frag t).
-  Proof.
-    intros. apply _.
-  Qed.
-End S.
-
-Class allDG Σ := AllDG {
-                      DG_invG :: invGS Σ;
-                      DG_memG :: gen_heapGS Addr Word Σ;
-                      DG_regG :: gen_heapGS Register Word Σ;
-                      DG_traceG :: traceG (list leak) Σ;
-                      DG_pcG :: traceG Word Σ;
-                      DG_progG :: traceG program Σ;
-                    }.
-
-
-
-(* invariants for memory, and a state interpretation for (mem,reg) *)
-Global Instance memG_irisG `{!allDG Σ} : irisGS asm_lang Σ := {
-  iris_invGS := DG_invG;
-  state_interp σ _ κs _ :=
-      ((@gen_heap_interp _ _ _ _ _ DG_regG (reg σ.1.2)) ∗
-         (@gen_heap_interp _ _ _ _ _ DG_memG (mem σ.1.2)) ∗
-    @tr_auth _ _ DG_traceG σ.2 ∗
-    @tr_auth _ _ DG_pcG (PC σ.1.2) ∗
-    @tr_auth _ _ DG_progG σ.1.1)%I;
-  fork_post _ := False%I;
-  num_laters_per_step _ := 0;
-  state_interp_mono _ _ _ _ := fupd_intro _ _
-}.
-
+From ASMinCoq Require Import CpdtTactics progLogHelper AsmGen.
 
 Section asm_lang_rules.
-  Context `{!allDG Σ}.
-  Context (γ ζ ξ : gname).
-(* Points to predicates for registers *)
-Print pointsto.
-Notation "r ↦ᵣ{ q } w" := (pointsto (hG := DG_regG) (L:=Register) (V:=Word) r q w)
-  (at level 20, q at level 50, format "r  ↦ᵣ{ q }  w") : bi_scope.
-Notation "r ↦ᵣ w" := (pointsto (hG := DG_regG) (L:=Register) (V:=Word) r (DfracOwn 1) w) (at level 20) : bi_scope.
+  Context `{!asmGS Σ}.
+  Import asm_lang.
 
-(* Points to predicates for memory *)
-Notation "a ↦ₐ{ q } w" := (pointsto (hG := DG_memG) (L:=Addr) (V:=Word) a q w)
-  (at level 20, q at level 50, format "a  ↦ₐ{ q }  w") : bi_scope.
-Notation "a ↦ₐ w" := (pointsto (hG := DG_memG) (L:=Addr) (V:=Word) a (DfracOwn 1) w) (at level 20) : bi_scope.
+  
+
+Global Program Instance asm_irisGS `{!asmGS Σ} : irisGS asm_lang Σ := {
+    iris_invGS := asmGS_invGS;
+    state_interp σ _ κs _ :=
+      ((@gen_heap_interp _ _ _ _ _ asm_regGS (reg σ.1.2)) ∗
+         (@gen_heap_interp _ _ _ _ _ asm_memGS (mem σ.1.2)) ∗
+         ll_auth σ.2 ∗
+         pc_auth (PC σ.1.2) ∗
+         prog_auth σ.1.1)%I;
+    fork_post _ := True%I;
+    num_laters_per_step n := n;
+  }.
+Next Obligation.
+  iIntros (Σ' ??? κs') "/= ($ & $ & H)".
+  iFrame. by iModIntro.
+Qed.
+
+  Notation "r ↦ᵣ{ q } w" := (pointsto (hG := asm_regGS) (L:=Register) (V:=Word) r q w)
+                              (at level 20, q at level 50, format "r  ↦ᵣ{ q }  w") : bi_scope.
+  Notation "r ↦ᵣ w" := (pointsto (hG := asm_regGS) (L:=Register) (V:=Word) r (DfracOwn 1) w) (at level 20) : bi_scope.
+
+  (* Points to predicates for memory *)
+  Notation "a ↦ₐ{ q } w" := (pointsto (hG := asm_memGS) (L:=Addr) (V:=Word) a q w)
+                              (at level 20, q at level 50, format "a  ↦ₐ{ q }  w") : bi_scope.
+  Notation "a ↦ₐ w" := (pointsto (hG := asm_memGS) (L:=Addr) (V:=Word) a (DfracOwn 1) w) (at level 20) : bi_scope.
 
 (* ------------------------- registers points-to --------------------------------- *)
 
@@ -169,82 +57,6 @@ Notation "a ↦ₐ w" := (pointsto (hG := DG_memG) (L:=Addr) (V:=Word) a (DfracO
     ([∗ map] k↦y ∈ {[r1 := w1]}, k ↦ᵣ y).
   Proof. rewrite big_sepM_singleton; auto. Qed.
 
-(*
-  Lemma regs_of_map_1 (r1: Register) (w1: Word) :
-    ([∗ map] k↦y ∈ {[r1 := w1]}, k ↦ᵣ y) -∗
-    r1 ↦ᵣ w1.
-  Proof. rewrite big_sepM_singleton; auto. Qed.
-
-  Lemma map_of_regs_2 (r1 r2: Register) (w1 w2: Word) :
-    r1 ↦ᵣ w1 -∗ r2 ↦ᵣ w2 -∗
-    ([∗ map] k↦y ∈ (<[r1:=w1]> (<[r2:=w2]> ∅)), k ↦ᵣ y) ∗ ⌜ r1 ≠ r2 ⌝.
-  Proof.
-    iIntros "H1 H2". iPoseProof (register_neq with "H1 H2") as "%".
-    rewrite !big_sepM_insert ?big_sepM_empty; eauto.
-    2: by apply lookup_insert_None; split; eauto.
-    iFrame. eauto.
-  Qed.
-
-  Lemma regs_of_map_2 (r1 r2: Register) (w1 w2: Word) :
-    r1 ≠ r2 →
-    ([∗ map] k↦y ∈ (<[r1:=w1]> (<[r2:=w2]> ∅)), k ↦ᵣ y) -∗
-    r1 ↦ᵣ w1 ∗ r2 ↦ᵣ w2.
-  Proof.
-    iIntros (?) "Hmap". rewrite !big_sepM_insert ?big_sepM_empty; eauto.
-    by iDestruct "Hmap" as "(? & ? & _)"; iFrame.
-    apply lookup_insert_None; split; eauto.
-  Qed.
-
-  Lemma map_of_regs_3 (r1 r2 r3: Register) (w1 w2 w3: Word) :
-    r1 ↦ᵣ w1 -∗ r2 ↦ᵣ w2 -∗ r3 ↦ᵣ w3 -∗
-    ([∗ map] k↦y ∈ (<[r1:=w1]> (<[r2:=w2]> (<[r3:=w3]> ∅))), k ↦ᵣ y) ∗
-     ⌜ r1 ≠ r2 ∧ r1 ≠ r3 ∧ r2 ≠ r3 ⌝.
-  Proof.
-    iIntros "H1 H2 H3".
-    iPoseProof (register_neq with "H1 H2") as "%".
-    iPoseProof (register_neq with "H1 H3") as "%".
-    iPoseProof (register_neq with "H2 H3") as "%".
-    rewrite !big_sepM_insert ?big_sepM_empty; simplify_map_eq; eauto.
-    iFrame. eauto.
-  Qed.
-
-  Lemma regs_of_map_3 (r1 r2 r3: Register) (w1 w2 w3: Word) :
-    r1 ≠ r2 → r1 ≠ r3 → r2 ≠ r3 →
-    ([∗ map] k↦y ∈ (<[r1:=w1]> (<[r2:=w2]> (<[r3:=w3]> ∅))), k ↦ᵣ y) -∗
-    r1 ↦ᵣ w1 ∗ r2 ↦ᵣ w2 ∗ r3 ↦ᵣ w3.
-  Proof.
-    iIntros (? ? ?) "Hmap". rewrite !big_sepM_insert ?big_sepM_empty; simplify_map_eq; eauto.
-    iDestruct "Hmap" as "(? & ? & ? & _)"; iFrame.
-  Qed.
-
-  Lemma map_of_regs_4 (r1 r2 r3 r4: Register) (w1 w2 w3 w4: Word) :
-    r1 ↦ᵣ w1 -∗ r2 ↦ᵣ w2 -∗ r3 ↦ᵣ w3 -∗ r4 ↦ᵣ w4 -∗
-    ([∗ map] k↦y ∈ (<[r1:=w1]> (<[r2:=w2]> (<[r3:=w3]> (<[r4:=w4]> ∅)))), k ↦ᵣ y) ∗
-     ⌜ r1 ≠ r2 ∧ r1 ≠ r3 ∧ r1 ≠ r4 ∧ r2 ≠ r3 ∧ r2 ≠ r4 ∧ r3 ≠ r4 ⌝.
-  Proof.
-    iIntros "H1 H2 H3 H4".
-    iPoseProof (register_neq with "H1 H2") as "%".
-    iPoseProof (register_neq with "H1 H3") as "%".
-    iPoseProof (register_neq with "H1 H4") as "%".
-    iPoseProof (register_neq with "H2 H3") as "%".
-    iPoseProof (register_neq with "H2 H4") as "%".
-    iPoseProof (register_neq with "H3 H4") as "%".
-    rewrite !big_sepM_insert ?big_sepM_empty; simplify_map_eq; eauto.
-    iFrame. eauto.
-  Qed.
-
-  Lemma regs_of_map_4 (r1 r2 r3 r4: Register) (w1 w2 w3 w4: Word) :
-    r1 ≠ r2 → r1 ≠ r3 → r1 ≠ r4 → r2 ≠ r3 → r2 ≠ r4 → r3 ≠ r4 →
-    ([∗ map] k↦y ∈ (<[r1:=w1]> (<[r2:=w2]> (<[r3:=w3]> (<[r4:=w4]> ∅)))), k ↦ᵣ y) -∗
-    r1 ↦ᵣ w1 ∗ r2 ↦ᵣ w2 ∗ r3 ↦ᵣ w3 ∗ r4 ↦ᵣ w4.
-  Proof.
-    intros. iIntros "Hmap". rewrite !big_sepM_insert ?big_sepM_empty; simplify_map_eq; eauto.
-    iDestruct "Hmap" as "(? & ? & ? & ? & _)"; iFrame.
-  Qed.
-*)
-
-  (* ------------------------- memory points-to --------------------------------- *)
-
   Lemma addr_dupl_false a w1 w2 :
     a ↦ₐ w1 -∗ a ↦ₐ w2 -∗ False.
   Proof.
@@ -256,8 +68,8 @@ Notation "a ↦ₐ w" := (pointsto (hG := DG_memG) (L:=Addr) (V:=Word) a (DfracO
 
   Lemma wp_halt pc prog ll E Φ :
     prog pc = Halt ->
-    tr_frag prog -∗ tr_frag pc -∗ tr_frag ll -∗
-    ▷ (tr_frag prog ∗ tr_frag pc ∗ tr_frag (NoLeak :: ll) -∗ Φ HaltedV) -∗
+    prog_frag prog -∗ pc_frag pc -∗ ll_frag ll -∗
+    ▷ (prog_frag prog ∗ pc_frag pc ∗ ll_frag (HaltLeak :: ll) -∗ Φ HaltedV) -∗
     WP (Instr Executable) @ E {{ v, Φ v }}.
   Proof.
     iIntros (prpcHalt) "Hprog Hpc Hll HΦ".
@@ -276,7 +88,7 @@ Notation "a ↦ₐ w" := (pointsto (hG := DG_memG) (L:=Addr) (V:=Word) a (DfracO
       inversion H; subst.
       simpl in *.
       rewrite prpcHalt in steps. rewrite prpcHalt. simpl in *. iFrame.
-      iPoseProof (trace_update _ (NoLeak :: ll) with "[$Hauthtrace $Hll]") as "H".
+      iPoseProof (trace_update _ (HaltLeak :: ll) with "[$Hauthtrace $Hll]") as "H".
       iMod "H". iModIntro. iNext. iModIntro.
       iDestruct "H" as "[Hauthll Hfragll]". iFrame.
       iSplitR.
@@ -284,145 +96,37 @@ Notation "a ↦ₐ w" := (pointsto (hG := DG_memG) (L:=Addr) (V:=Word) a (DfracO
       iApply "HΦ". iFrame.
   Qed.
 
-  Fixpoint regs_from_inputs {n : nat} (inputs : vec (Word + Register) n) : gset Register :=
-    match inputs with
-    | [# ] => ∅
-    | wr ::: inputs' => match wr with
-                        | inl _ => regs_from_inputs inputs'
-                        | inr r => {[ r ]} ∪ regs_from_inputs inputs'
-                        end
-    end.
-
-  Fixpoint replace_in_inputs {n : nat} (words : list Word) (inputs : vec (Word + Register) n)
-    : vec Word n :=
-    match inputs, words with
-    | Vector.nil, _ => Vector.nil
-    | Vector.cons input inputs', [] => match input with
-                                | inl w => Vector.cons w (replace_in_inputs words inputs')
-                                | inr _ => Vector.cons (word 0) (replace_in_inputs words inputs')
-                                end
-    | Vector.cons input inputs', w' :: words' => match input with
-                                | inl w => Vector.cons w (replace_in_inputs words inputs')
-                                | inr _ => Vector.cons w' (replace_in_inputs words' inputs')
-                                end
-    end.
-
-  Definition regs_of_argument (arg: Word + Register) : gset Register :=
-  match arg with
-  | inl _ => ∅
-  | inr r => {[ r ]}
-  end.
-
-Definition regs_of (i: instr): gset Register :=
-match i with
-    | Computation inputs rres f_result => {[ rres ]} ∪ regs_from_inputs inputs
-    | ControlFlow inputs dst f_condition => regs_of_argument dst ∪ regs_from_inputs inputs
-    | Load rres rsrc => {[ rres; rsrc ]}
-    | Store rdst src => {[ rdst ]} ∪ regs_of_argument src
-    | _ => ∅
-end.
-
-Lemma indom_regs_incl D (regs regs': Reg) :
-  D ⊆ dom regs →
-  regs ⊆ regs' →
-  ∀ r, r ∈ D →
-       ∃ (w:Word), (regs !! r = Some w) ∧ (regs' !! r = Some w).
-Proof.
-  intros * HD Hincl rr Hr.
-  assert (is_Some (regs !! rr)) as [w Hw].
-  { eapply @elem_of_dom with (D := gset Register). typeclasses eauto.
-    eapply elem_of_subseteq; eauto. }
-  exists w. split; auto. eapply lookup_weaken; eauto.
-Qed.
-
-Lemma indom_regs_incl_default D (regs regs': Reg) :
-  D ⊆ dom regs →
-  regs ⊆ regs' →
-  ∀ r, r ∈ D →
-       ∃ (w:Word), (regs !!! r = w) ∧ (regs' !!! r = w).
-Proof.
-  intros * HD Hincl rr Hr.
-  specialize (indom_regs_incl _ _ _ HD Hincl rr Hr) as [w [Hw Hw']].
-  unfold "!!!". unfold lookup_total_register. unfold map_lookup_total. unfold default. simpl. rewrite Hw.
-  exists w. split; auto. rewrite (lookup_weaken _ _ _ _ Hw Hincl). reflexivity.
-Qed.
-
-Lemma gen_heap_update_inSepM :
-    ∀ {L V : Type} {EqDecision0 : EqDecision L}
-      {H : Countable L} {Σ : gFunctors}
-      {gen_heapG0 : gen_heapGS L V Σ}
-      (σ σ' : gmap L V) (l : L) (v : V),
-      is_Some (σ' !! l) →
-      gen_heap_interp σ
-      -∗ ([∗ map] k↦y ∈ σ', pointsto k (DfracOwn 1) y)
-      ==∗ gen_heap_interp (<[l:=v]> σ)
-          ∗ [∗ map] k↦y ∈ (<[l:=v]> σ'), pointsto k (DfracOwn 1) y.
+  Lemma twp_halt pc prog ll E Φ :
+    prog pc = Halt ->
+    prog_frag prog -∗ pc_frag pc -∗ ll_frag ll -∗
+    (prog_frag prog ∗ pc_frag pc ∗ ll_frag (HaltLeak :: ll) -∗ Φ HaltedV) -∗
+    twp NotStuck E (Instr Executable) Φ.
   Proof.
-    intros * Hσ'. destruct Hσ'.
-    rewrite (big_sepM_delete _ σ' l) //. iIntros "Hh [Hl Hmap]".
-    iMod (gen_heap_update with "Hh Hl") as "[Hh Hl]". iModIntro.
-    iSplitL "Hh"; eauto.
-    rewrite (big_sepM_delete _ (<[l:=v]> σ') l).
-    { rewrite delete_insert_delete. iFrame. }
-    rewrite lookup_insert //.
+    iIntros (prpcHalt) "Hprog Hpc Hll HΦ".
+    iApply twp_lift_atomic_step_no_fork_fupd; auto.
+    iIntros (σ ns κs nt) "(Hauthreg & Hauthmem & Hauthtrace & Hauthpc & Hauthprog)".
+    destruct σ as [s ll'].
+    simpl.
+    iDestruct (@trace_full_frag_eq with "Hauthtrace Hll") as %?; subst; auto.
+    iDestruct (@trace_full_frag_eq with "Hauthpc Hpc") as %?; subst; auto.
+    iDestruct (@trace_full_frag_eq with "Hauthprog Hprog") as %?; subst; auto.
+    iModIntro.
+    iSplitR.
+    - iPureIntro. apply normal_always_reducible_no_obs.
+    - iIntros (κ e2 σ2 efs) "%steps".
+      inversion steps; subst; simpl in *.
+      inversion H; subst.
+      simpl in *.
+      rewrite prpcHalt in steps. rewrite prpcHalt. simpl in *. iFrame.
+      iPoseProof (trace_update _ (HaltLeak :: ll) with "[$Hauthtrace $Hll]") as "H".
+      iMod "H". iModIntro.
+      iDestruct "H" as "[Hauthll Hfragll]". iFrame.
+      iSplitR.
+      { iPureIntro; reflexivity. }
+      iSplitR.
+      { iPureIntro; reflexivity. }
+      iApply "HΦ". iFrame.
   Qed.
-
-  Lemma gen_heap_valid_inSepM':
-    ∀ (L V : Type) (EqDecision0 : EqDecision L) (H : Countable L)
-      (Σ : gFunctors) (gen_heapG0 : gen_heapGS L V Σ)
-      (σ σ' : gmap L V) (q : Qp),
-      gen_heap_interp σ -∗
-      ([∗ map] k↦y ∈ σ', pointsto k (DfracOwn q) y) -∗
-      ⌜forall (l: L) (v: V), σ' !! l = Some v → σ !! l = Some v⌝.
-  Proof.
-    intros *. iIntros "? Hmap" (l v Hσ').
-    rewrite (big_sepM_delete _ σ' l) //. iDestruct "Hmap" as "[? ?]".
-    iApply (gen_heap_valid with "[$]"). eauto.
-  Qed.
-
-  Lemma gen_heap_valid_inclSepM:
-    ∀ (L V : Type) (EqDecision0 : EqDecision L) (H : Countable L)
-      (Σ : gFunctors) (gen_heapG0 : gen_heapGS L V Σ)
-      (σ σ' : gmap L V) (q : Qp),
-      gen_heap_interp σ -∗
-      ([∗ map] k↦y ∈ σ', pointsto k (DfracOwn q) y) -∗
-      ⌜σ' ⊆ σ⌝.
-  Proof.
-    intros *. iIntros "Hσ Hmap".
-    iDestruct (gen_heap_valid_inSepM' with "Hσ Hmap") as "#H".
-    iDestruct "H" as %Hincl. iPureIntro. intro l.
-    unfold option_relation.
-    destruct (σ' !! l) eqn:HH'; destruct (σ !! l) eqn:HH; naive_solver.
-  Qed.
-
-Lemma inputs_are_enough {B : Type} {n : nat} regs regs' (f_result : vec Word n -> B) (inputs : vec (Word + Register) n)
-  (inputs_in_regs : regs_from_inputs inputs ⊆ dom regs)
-  (regs_in_regs' : regs ⊆ regs') :
-  f_result (inputs_from_inputnatregs regs inputs) = f_result (inputs_from_inputnatregs regs' inputs).
-Proof.
-  induction inputs.
-  - reflexivity.
-  - destruct h.
-    + simpl. unfold regs_from_inputs in inputs_in_regs. simpl in inputs_in_regs.
-      apply (IHinputs (fun inputs' => f_result (w ::: inputs'))) in inputs_in_regs.
-      apply inputs_in_regs.
-    + simpl. specialize (indom_regs_incl_default _ _ _ inputs_in_regs regs_in_regs' r) as Hri.
-      destruct Hri.
-      { set_solver+. }
-      destruct H as [Hregs Hregs']. rewrite Hregs Hregs'.
-      simpl in inputs_in_regs. apply union_subseteq in inputs_in_regs. 
-      apply (IHinputs (fun inputs' => f_result (x ::: inputs'))).
-      destruct inputs_in_regs as [_ ->]. reflexivity.
-Qed.
-
-Lemma regs_of_computation {n : nat} (inputs : vec (Word + Register) n)
-    (rres : Register) (f_result : vec Word n -> Word) i :
-    i = Computation inputs rres f_result ->
-    regs_of i = {[ rres ]} ∪ regs_from_inputs inputs.
-Proof.
-  intros. subst.
-  reflexivity.
-Qed.
 
 Inductive Computation_spec {n : nat} (inputs : vec (Word + Register) n) (rres : Register) f_result (regs : Reg) (regs' : Reg) : Prop :=
   | Computation_spec_success vn  :
@@ -435,9 +139,9 @@ Lemma wp_computation {n : nat} regs regs' pc prog ll
   prog pc = Computation inputs rres f_result ->
   regs_of (Computation inputs rres f_result) ⊆ dom regs →
   Computation_spec (n := n) inputs rres f_result regs regs' ->
-  tr_frag prog -∗ tr_frag pc -∗
-  tr_frag ll -∗ ([∗ map] k↦y ∈ regs, k ↦ᵣ y) -∗
-    ▷ ((tr_frag prog ∗ tr_frag (incr_word pc) ∗ tr_frag (NoLeak :: ll) ∗
+  prog_frag prog -∗ pc_frag pc -∗
+  ll_frag ll -∗ ([∗ map] k↦y ∈ regs, k ↦ᵣ y) -∗
+    ▷ ((prog_frag prog ∗ pc_frag (incr_word pc) ∗ ll_frag (ComputationLeak f_result :: ll) ∗
     [∗ map] k↦y ∈ regs', k ↦ᵣ y) -∗ Φ NextIV) -∗
     WP (Instr Executable) @ E {{ v, Φ v }}.
   Proof.
@@ -450,7 +154,7 @@ Lemma wp_computation {n : nat} regs regs' pc prog ll
     iDestruct (@trace_full_frag_eq with "Hauthtrace Hll") as %?; subst; auto.
     iDestruct (@trace_full_frag_eq with "Hauthpc Hpc") as %?; subst; auto.
     iDestruct (@trace_full_frag_eq with "Hauthprog Hprog") as %?; subst; auto.
-    iPoseProof (trace_update _ (NoLeak :: ll) with "[$Hauthtrace $Hll]") as "H1".
+    iPoseProof (trace_update _ (ComputationLeak f_result :: ll) with "[$Hauthtrace $Hll]") as "H1".
     iPoseProof (trace_update _ (incr_word (PC (s.2))) with "[$Hauthpc $Hpc]") as "H2".
 
     iDestruct (gen_heap_valid_inclSepM with "Hreg HlistOfRegs") as %Hregs.
@@ -475,17 +179,58 @@ Lemma wp_computation {n : nat} regs regs' pc prog ll
       iFrame.
       iSplitR; try (iPureIntro; reflexivity).
       iApply "HΦ"; iFrame.
-      rewrite (inputs_are_enough regs (reg φ)); auto.
+      rewrite (inputs_are_enough _ Hregs); auto.
       apply union_subseteq in regs_subset as [_ ->]; reflexivity.
 Qed.
 
-Lemma regs_of_control_flow {n : nat} (inputs : vec (Word + Register) n)
-    (dst : Word + Register) (f_condition : vec Word n -> bool) i :
-    i = ControlFlow inputs dst f_condition ->
-    regs_of i = regs_of_argument dst ∪ regs_from_inputs inputs.
-Proof.
-  intros. subst.
-  reflexivity.
+
+Lemma twp_computation {n : nat} regs regs' pc prog ll
+    (inputs : vec (Word + Register) n) rres f_result Φ E :
+  prog pc = Computation inputs rres f_result ->
+  regs_of (Computation inputs rres f_result) ⊆ dom regs →
+  Computation_spec (n := n) inputs rres f_result regs regs' ->
+  prog_frag prog -∗ pc_frag pc -∗
+  ll_frag ll -∗ ([∗ map] k↦y ∈ regs, k ↦ᵣ y) -∗
+                                                ((prog_frag prog -∗ pc_frag (incr_word pc) -∗ ll_frag (ComputationLeak f_result :: ll) -∗
+    [∗ map] k↦y ∈ regs', k ↦ᵣ y) -∗ Φ NextIV) -∗
+    twp NotStuck E (Instr Executable) Φ.
+  Proof.
+    iIntros (prpcHalt regs_subset Hcomp) "Hprog Hpc Hll HlistOfRegs HΦ".
+    inversion Hcomp; subst; clear Hcomp.
+    iApply twp_lift_atomic_step_no_fork_fupd; auto.
+    iIntros (σ ns κs nt) "(Hreg & Hmem & Hauthtrace & Hauthpc & Hauthprog)".
+    destruct σ as [s ll']. 
+    simpl.
+    iDestruct (@trace_full_frag_eq with "Hauthtrace Hll") as %?; subst; auto.
+    iDestruct (@trace_full_frag_eq with "Hauthpc Hpc") as %?; subst; auto.
+    iDestruct (@trace_full_frag_eq with "Hauthprog Hprog") as %?; subst; auto.
+    iPoseProof (trace_update _ (ComputationLeak f_result :: ll) with "[$Hauthtrace $Hll]") as "H1".
+    iPoseProof (trace_update _ (incr_word (PC (s.2))) with "[$Hauthpc $Hpc]") as "H2".
+
+    iDestruct (gen_heap_valid_inclSepM with "Hreg HlistOfRegs") as %Hregs.
+    specialize (indom_regs_incl _ _ _ regs_subset Hregs) as Hri.
+    destruct (Hri rres) as [wdst [H'dst Hdst]]. by set_solver+.        
+    iMod "H1". iMod "H2". iModIntro.
+
+    iDestruct "H1" as "[Hauthll Hfragll]". iDestruct "H2" as "[Hauthpc Hfragpc]".
+    iSplitR.
+    - iPureIntro. apply normal_always_reducible_no_obs.
+    - iIntros (κ e2 σ2 efs) "%steps".
+      inversion steps; subst; simpl in *.
+      inversion H; subst.
+      simpl in *.
+      rewrite prpcHalt in steps. rewrite prpcHalt. simpl in *.     
+      iFrame.
+      unfold incr_PC. rewrite -(update_pc_no_change_reg).
+      rewrite reg_is_updated_value.
+      iMod ((gen_heap_update_inSepM _ _ rres) with "Hreg HlistOfRegs") as "[Hr Hmap]".
+      { eauto.  }
+      iModIntro.
+      iFrame.
+      do 2 (iSplitR; try (iPureIntro; reflexivity)).
+      iApply "HΦ"; iFrame.
+      rewrite (inputs_are_enough _ Hregs); auto.
+      apply union_subseteq in regs_subset as [_ ->]; reflexivity.
 Qed.
 
 Inductive Control_flow_spec {n : nat} (inputs : vec (Word + Register) n) (dst : Word + Register) f_condition (regs : Reg) (pc pc' : Word) : Prop :=
@@ -504,10 +249,10 @@ Lemma wp_control_flow {n : nat} regs pc pc' prog ll (inputs : vec (Word + Regist
   prog pc = ControlFlow inputs dst f_condition ->
   Control_flow_spec inputs dst f_condition regs pc pc' ->
   regs_of (ControlFlow inputs dst f_condition) ⊆ dom regs →
-  tr_frag prog -∗ tr_frag pc -∗ tr_frag ll -∗
+  prog_frag prog -∗ pc_frag pc -∗ ll_frag ll -∗
   ([∗ map] k↦y ∈ regs, k ↦ᵣ y) -∗
-  ▷(tr_frag prog ∗ tr_frag pc' ∗
-      tr_frag (ControlFlowLeak (f_condition (inputs_from_inputnatregs regs inputs)) :: ll) ∗
+  ▷(prog_frag prog ∗ pc_frag pc' ∗
+      ll_frag (ControlFlowLeak pc' :: ll) ∗
     ([∗ map] k↦y ∈ regs, k ↦ᵣ y) -∗ Φ NextIV) -∗
     WP (Instr Executable) @ E {{ v, Φ v }}.
 Proof.
@@ -530,18 +275,65 @@ Proof.
       rewrite prpcHalt in steps. rewrite prpcHalt. simpl in *.
       inversion HcontrolFlow; subst; clear HcontrolFlow.
       all: apply union_subseteq in regs_subset as [dst_subset inputs_subset].
-      all: rewrite (inputs_are_enough _ (reg φ)) in H1; auto.
+      all: rewrite (inputs_are_enough _ Hregs) in H1; auto.
       all: destruct (f_condition (inputs_from_inputnatregs (reg φ) inputs)) as [|] eqn:Hcondition; try congruence.
-      all: iPoseProof (trace_update _ (ControlFlowLeak (f_condition (inputs_from_inputnatregs (reg φ) inputs)) :: ll) with "[$Hauthtrace $Hll]") as "H1".
+      1: iPoseProof (trace_update _ (ControlFlowLeak (wordreg_to_word (reg φ) dst) :: ll) with "[$Hauthtrace $Hll]") as "H1".
+      2: iPoseProof (trace_update _ (ControlFlowLeak (PC (incr_PC φ)) :: ll) with "[$Hauthtrace $Hll]") as "H1".
       1: iPoseProof (trace_update _ (wordreg_to_word (reg φ) dst) with "[$Hauthpc $Hpc]") as "H2".
       2: iPoseProof (trace_update _ (incr_word (PC φ)) with "[$Hauthpc $Hpc]") as "H2".
-      all: iMod "H1"; iMod "H2"; iDestruct "H1" as "[Hauthll Hfragll]"; iDestruct "H2" as "[Hauthpc Hfragpc]";
-      rewrite Hcondition; iFrame.
+      all: iMod "H1"; iMod "H2"; iDestruct "H1" as "[Hauthll Hfragll]"; iDestruct "H2" as "[Hauthpc Hfragpc]"; iFrame.
       all: iModIntro; iNext; iModIntro.
       all: iSplitR; try (iPureIntro; reflexivity).
       all: iApply "HΦ".
-      all: assert ((f_condition (inputs_from_inputnatregs regs inputs) = f_condition (inputs_from_inputnatregs (reg φ) inputs))) as Hreg_regφ;
-      try (apply (inputs_are_enough regs (reg φ)); auto; apply union_subseteq in regs_subset as [_ ->]; reflexivity); rewrite Hreg_regφ Hcondition.
+      all: iFrame.
+      destruct dst; iFrame.
+      specialize (indom_regs_incl_default _ _ _ dst_subset Hregs r) as Hri.
+      destruct Hri as [w [Hw Hw']]. {set_solver. }
+      simpl.
+      rewrite Hw Hw'. iFrame.
+Qed.
+
+
+Lemma twp_control_flow {n : nat} regs pc pc' prog ll (inputs : vec (Word + Register) n) dst f_condition E Φ :
+  prog pc = ControlFlow inputs dst f_condition ->
+  Control_flow_spec inputs dst f_condition regs pc pc' ->
+  regs_of (ControlFlow inputs dst f_condition) ⊆ dom regs →
+  prog_frag prog -∗ pc_frag pc -∗ ll_frag ll -∗
+  ([∗ map] k↦y ∈ regs, k ↦ᵣ y) -∗
+  (prog_frag prog ∗ pc_frag pc' ∗
+      ll_frag (ControlFlowLeak pc' :: ll) ∗
+    ([∗ map] k↦y ∈ regs, k ↦ᵣ y) -∗ Φ NextIV) -∗
+    twp NotStuck E (Instr Executable) Φ.
+Proof.
+    iIntros (prpcHalt HcontrolFlow regs_subset) "Hprog Hpc Hll HlistOfRegs HΦ".
+    iApply twp_lift_atomic_step_no_fork_fupd; auto.
+    iIntros (σ ns κs nt) "(Hreg & Hmem & Hauthtrace & Hauthpc & Hauthprog)".
+    destruct σ as [s ll'].
+    simpl.
+    iDestruct (@trace_full_frag_eq with "Hauthtrace Hll") as %?; subst; auto.
+    iDestruct (@trace_full_frag_eq with "Hauthpc Hpc") as %?; subst; auto.
+    iDestruct (@trace_full_frag_eq with "Hauthprog Hprog") as %?; subst; auto.
+    iDestruct (gen_heap_valid_inclSepM with "Hreg HlistOfRegs") as %Hregs.   
+    iModIntro.
+    iSplitR.
+    - iPureIntro. apply normal_always_reducible_no_obs.
+    - iIntros (κ e2 σ2 efs) "%steps".
+      inversion steps; subst; simpl in *.
+      inversion H; subst.
+      simpl in *.
+      rewrite prpcHalt in steps. rewrite prpcHalt. simpl in *.
+      inversion HcontrolFlow; subst; clear HcontrolFlow.
+      all: apply union_subseteq in regs_subset as [dst_subset inputs_subset].
+      all: rewrite (inputs_are_enough _ Hregs) in H1; auto.
+      all: destruct (f_condition (inputs_from_inputnatregs (reg φ) inputs)) as [|] eqn:Hcondition; try congruence.
+      1: iPoseProof (trace_update _ (ControlFlowLeak (wordreg_to_word (reg φ) dst) :: ll) with "[$Hauthtrace $Hll]") as "H1".
+      2: iPoseProof (trace_update _ (ControlFlowLeak (PC (incr_PC φ)) :: ll) with "[$Hauthtrace $Hll]") as "H1".
+      1: iPoseProof (trace_update _ (wordreg_to_word (reg φ) dst) with "[$Hauthpc $Hpc]") as "H2".
+      2: iPoseProof (trace_update _ (incr_word (PC φ)) with "[$Hauthpc $Hpc]") as "H2".
+      all: iMod "H1"; iMod "H2"; iDestruct "H1" as "[Hauthll Hfragll]"; iDestruct "H2" as "[Hauthpc Hfragpc]"; iFrame.
+      all: iModIntro.
+      all: do 2 (iSplitR; try (iPureIntro; reflexivity)).
+      all: iApply "HΦ".
       all: iFrame.
       destruct dst; iFrame.
       specialize (indom_regs_incl_default _ _ _ dst_subset Hregs r) as Hri.
@@ -553,11 +345,11 @@ Qed.
 Lemma wp_load {n : nat} pc prog ll regs rres rsrc v E Φ :
   prog pc = Load rres rsrc ->
   regs_of (Load rres rsrc) ⊆ dom regs →
-  tr_frag prog -∗ tr_frag pc -∗ tr_frag ll -∗
+  prog_frag prog -∗ pc_frag pc -∗ ll_frag ll -∗
       ([∗ map] k↦y ∈ regs, k ↦ᵣ y) -∗
       word_to_addr (regs !!! rsrc) ↦ₐ v -∗
-  ▷(tr_frag prog ∗ tr_frag (incr_word pc) ∗
-      tr_frag (LoadLeak (word_to_addr (regs !!! rsrc)) :: ll) ∗
+  ▷(prog_frag prog ∗ pc_frag (incr_word pc) ∗
+      ll_frag (LoadLeak (word_to_addr (regs !!! rsrc)) :: ll) ∗
       ([∗ map] k↦y ∈ <[ rres := v ]>regs, k ↦ᵣ y) -∗ Φ NextIV) -∗
   WP (Instr Executable) @ E {{ v, Φ v }}.
   Proof.
@@ -588,7 +380,7 @@ Lemma wp_load {n : nat} pc prog ll regs rres rsrc v E Φ :
     iMod ((gen_heap_update_inSepM _ _ rres) with "Hreg HlistOfRegs") as "[Hr Hmap]".
     { eapply @elem_of_dom with (D := gset Register). typeclasses eauto.
     eapply elem_of_subseteq; eauto. set_solver. }
-    iPoseProof (gen_heap_valid (gen_heapGS0 := DG_memG) with "Hmem Haddrv") as "%Hmem'".
+    iPoseProof (gen_heap_valid (gen_heapGS0 := asm_memGS) with "Hmem Haddrv") as "%Hmem'".
     iModIntro. iNext. iModIntro. iFrame.
     iSplitR.
     { iPureIntro. reflexivity. }
@@ -603,14 +395,67 @@ Lemma wp_load {n : nat} pc prog ll regs rres rsrc v E Φ :
     rewrite Hmem''. iFrame.
 Qed.
 
+
+Lemma twp_load {n : nat} pc prog ll regs rres rsrc v E Φ :
+  prog pc = Load rres rsrc ->
+  regs_of (Load rres rsrc) ⊆ dom regs →
+  prog_frag prog -∗ pc_frag pc -∗ ll_frag ll -∗
+      ([∗ map] k↦y ∈ regs, k ↦ᵣ y) -∗
+      word_to_addr (regs !!! rsrc) ↦ₐ v -∗
+  (prog_frag prog ∗ pc_frag (incr_word pc) ∗
+      ll_frag (LoadLeak (word_to_addr (regs !!! rsrc)) :: ll) ∗
+      ([∗ map] k↦y ∈ <[ rres := v ]>regs, k ↦ᵣ y) -∗ Φ NextIV) -∗
+  twp NotStuck E (Instr Executable) Φ.
+  Proof.
+    iIntros (prpcHalt regs_subset) "Hprog Hpc Hll HlistOfRegs Haddrv HΦ".
+    iApply twp_lift_atomic_step_no_fork_fupd; auto.
+    iIntros (σ ns κs nt) "(Hreg & Hmem & Hauthtrace & Hauthpc & Hauthprog)".
+    destruct σ as [s ll'].
+    simpl.
+    iDestruct (@trace_full_frag_eq with "Hauthtrace Hll") as %?; subst; auto.
+    iDestruct (@trace_full_frag_eq with "Hauthpc Hpc") as %?; subst; auto.
+    iDestruct (@trace_full_frag_eq with "Hauthprog Hprog") as %?; subst; auto.
+    iDestruct (gen_heap_valid_inclSepM with "Hreg HlistOfRegs") as %Hregs.
+    iModIntro.
+
+    iSplitR.
+    { iPureIntro. apply normal_always_reducible_no_obs. }
+    iIntros (κ e2 σ2 efs) "%steps".
+    inversion steps; subst; simpl in *.
+    inversion H; subst.
+    simpl in *.
+    rewrite prpcHalt in steps. rewrite prpcHalt. simpl in *.
+
+    iPoseProof (trace_update _ (LoadLeak (word_to_addr (reg φ !!! rsrc)) :: ll) with "[$Hauthtrace $Hll]") as "H1".
+    iPoseProof (trace_update _ (incr_word (PC φ)) with "[$Hauthpc $Hpc]") as "H2".
+    iMod "H1"; iMod "H2"; iDestruct "H1" as "[Hauthll Hfragll]"; iDestruct "H2" as "[Hauthpc Hfragpc]".
+    
+    unfold incr_PC. rewrite -update_pc_no_change_reg. rewrite reg_is_updated_value.
+    iMod ((gen_heap_update_inSepM _ _ rres) with "Hreg HlistOfRegs") as "[Hr Hmap]".
+    { eapply @elem_of_dom with (D := gset Register). typeclasses eauto.
+    eapply elem_of_subseteq; eauto. set_solver. }
+    iPoseProof (gen_heap_valid (gen_heapGS0 := asm_memGS) with "Hmem Haddrv") as "%Hmem'".
+    iModIntro. iFrame.
+    do 2 (iSplitR; try (iPureIntro; reflexivity)).
+    
+    iApply "HΦ"; iFrame.
+    specialize (indom_regs_incl_default _ _ _ regs_subset Hregs rsrc) as Hri.
+    destruct Hri as [w [Hw Hw']]. { set_solver. }
+    rewrite Hw. rewrite Hw'. iFrame.
+    rewrite Hw in Hmem'. unfold word_to_addr in Hmem'.
+    assert (mem φ !!! (word_to_addr w) = v) as Hmem''.
+    { unfold "!!!". unfold lookup_total_memory. unfold map_lookup_total. unfold default. rewrite Hmem'. reflexivity. }
+    rewrite Hmem''. iFrame.
+Qed.
+
 Lemma wp_store pc prog ll regs rdst src v E Φ :
   prog pc = Store rdst src ->
   regs_of (Store rdst src) ⊆ dom regs →
-  tr_frag prog -∗ tr_frag pc -∗ tr_frag ll -∗
+  prog_frag prog -∗ pc_frag pc -∗ ll_frag ll -∗
       ([∗ map] k↦y ∈ regs, k ↦ᵣ y) -∗
       word_to_addr (regs !!! rdst) ↦ₐ v -∗
-  ▷(tr_frag prog ∗ tr_frag (incr_word pc) ∗
-      tr_frag (StoreLeak (word_to_addr (wordreg_to_word regs src)) :: ll) ∗
+  ▷(prog_frag prog ∗ pc_frag (incr_word pc) ∗
+      ll_frag (StoreLeak (word_to_addr (wordreg_to_word regs src)) :: ll) ∗
       ([∗ map] k↦y ∈ regs, k ↦ᵣ y) ∗
       word_to_addr (regs !!! rdst) ↦ₐ wordreg_to_word regs src -∗
     Φ NextIV) -∗
@@ -658,16 +503,62 @@ Lemma wp_store pc prog ll regs rdst src v E Φ :
     all: destruct Hri as [w1 [Hw1 Hw1']]; try (rewrite Hw1 Hw1'; iFrame); try set_solver.
 Qed.
 
-Definition test_prog_not_constant_time (high_input : nat) :=
-  list_prog_to_prog [Add (register 0) (inl (word high_input)) (inl (word high_input)); Jnz (inr (register 0)) (inl (word 3))].
 
-Definition loopify (e : expr) : expr :=
-  match e with
-  | Instr cf => Loop cf
-  | Loop cf => Loop cf
-  end.
+Lemma twp_store pc prog ll regs rdst src v E Φ :
+  prog pc = Store rdst src ->
+  regs_of (Store rdst src) ⊆ dom regs →
+  prog_frag prog -∗ pc_frag pc -∗ ll_frag ll -∗
+      ([∗ map] k↦y ∈ regs, k ↦ᵣ y) -∗
+      word_to_addr (regs !!! rdst) ↦ₐ v -∗
+  (prog_frag prog ∗ pc_frag (incr_word pc) ∗
+      ll_frag (StoreLeak (word_to_addr (wordreg_to_word regs src)) :: ll) ∗
+      ([∗ map] k↦y ∈ regs, k ↦ᵣ y) ∗
+      word_to_addr (regs !!! rdst) ↦ₐ wordreg_to_word regs src -∗
+    Φ NextIV) -∗
+    twp NotStuck E (Instr Executable) Φ.
+  Proof.
+    iIntros (prpcHalt regs_subset) "Hprog Hpc Hll HlistOfRegs Haddrv HΦ".
+    iApply twp_lift_atomic_step_no_fork_fupd; auto.
+    iIntros (σ ns κs nt) "(Hreg & Hmem & Hauthtrace & Hauthpc & Hauthprog)".
+    destruct σ as [s ll'].
+    simpl.
+    iDestruct (@trace_full_frag_eq with "Hauthtrace Hll") as %?; subst; auto.
+    iDestruct (@trace_full_frag_eq with "Hauthpc Hpc") as %?; subst; auto.
+    iDestruct (@trace_full_frag_eq with "Hauthprog Hprog") as %?; subst; auto.
+    iDestruct (gen_heap_valid_inclSepM with "Hreg HlistOfRegs") as %Hregs.
+    iModIntro.
 
-#[export] Instance language_ctx_loopify : LanguageCtx loopify.
+    iSplitR.
+    { iPureIntro. apply normal_always_reducible_no_obs. }
+    iIntros (κ e2 σ2 efs) "%steps".
+    inversion steps; subst; simpl in *.
+    inversion H; subst.
+    simpl in *.
+    rewrite prpcHalt in steps. rewrite prpcHalt. simpl in *.
+
+    iPoseProof (trace_update _ (StoreLeak ((word_to_addr (wordreg_to_word regs src))) :: ll) with "[$Hauthtrace $Hll]") as "H1".
+    iPoseProof (trace_update _ (incr_word (PC φ)) with "[$Hauthpc $Hpc]") as "H2".
+    iMod "H1"; iMod "H2"; iDestruct "H1" as "[Hauthll Hfragll]"; iDestruct "H2" as "[Hauthpc Hfragpc]".
+    
+    unfold incr_PC. rewrite -update_pc_no_change_reg. rewrite -update_mem_no_change_reg.
+    iPoseProof (gen_heap_valid with "Hmem Haddrv") as "%Hmem'".
+    
+    iMod ((gen_heap_update _ (word_to_addr (regs !!! rdst))) with "Hmem Haddrv") as "[Hr Hmap]".
+    specialize (indom_regs_incl_default _ _ _ regs_subset Hregs rdst) as Hri.
+    destruct Hri as [w [Hw Hw']]. { set_solver. }
+    rewrite Hw Hw'.
+
+    iModIntro. clear. iFrame.
+    do 2 (iSplitR; try (iPureIntro; reflexivity)).
+    
+    iSplitL "Hauthll".
+    all: destruct src; simpl; iFrame.
+    all: try iApply "HΦ"; iFrame.
+    all: specialize (indom_regs_incl_default _ _ _ regs_subset Hregs r) as Hri.
+    all: destruct Hri as [w1 [Hw1 Hw1']]; try (rewrite Hw1 Hw1'; iFrame); try set_solver.
+Qed.
+
+#[export] Instance language_ctx_loopify : @LanguageCtx asm_lang loopify.
 Proof.
   constructor.
   - intros e e_is_None.
@@ -724,13 +615,13 @@ Qed.
 
 
 Lemma wp_test :
-  {{{ tr_frag (test_prog_not_constant_time 2) ∗
-      tr_frag (word 0) ∗ tr_frag [] ∗
+  {{{ prog_frag (test_prog_not_constant_time 2) ∗
+      pc_frag (word 0) ∗ ll_frag [] ∗
       register 0 ↦ᵣ word 0 }}}
       (Loop Executable)
-  {{{ RET LoopHaltedV; tr_frag (test_prog_not_constant_time 2)
-      ∗ tr_frag (word 3) ∗
-      tr_frag ([NoLeak; ControlFlowLeak true; NoLeak]) ∗
+  {{{ RET LoopHaltedV; prog_frag (test_prog_not_constant_time 2)
+      ∗ pc_frag (word 3) ∗
+      ll_frag ([HaltLeak; ControlFlowLeak (word 3); AddLeak]) ∗
       register 0 ↦ᵣ word 4
      }}}.
 Proof.
@@ -752,7 +643,7 @@ Proof.
   iApply wp_bind_loop_executable.
   iApply (wp_halt with "[$Hprog] [$Hpc] [$Hll]"); try reflexivity.
   iNext. iIntros "(Hprog & Hpc & Hll)". simpl.
-  iApply wp_loop_halted. iApply "HΦ". rewrite lookup_total_insert. iFrame.
+  iApply wp_loop_halted. iApply "HΦ". iFrame.
   iPoseProof (big_sepM_insert with "Hmap") as "[H1 H2]".
   { constructor. }
   iFrame.
