theories/progLog2.v
@@ -4,64 +4,76 @@ From iris.program_logic Require Export weakestpre ectx_lifting total_weakestpre.
 From iris.algebra Require Import frac auth gmap excl.
 From Coq.Lists Require Import List.
 From ASMinCoq Require Import CpdtTactics.
-From ASMinCoq Require Import AsmGen progLog.
+From ASMinCoq Require Import AsmGen progLog dwp lifting.
 
 Class binDG Σ := BinDG {
-  bin_invG :> invGS Σ;
-  fst_memG :> gen_heapGS Addr Word Σ;
-  snd_memG :> gen_heapGS Addr Word Σ;
-  fst_regG :> gen_heapGS Register Word Σ;
-  snd_regG :> gen_heapGS Register Word Σ;
-  fst_traceG :: traceG (list leak) Σ;
+  bin_invG :: invGS Σ;
+  fst_memG :: gen_heapGS Addr Word Σ;
+  snd_memG :: gen_heapGS Addr Word Σ;
+  fst_regG :: gen_heapGS Register Word Σ;
+  snd_regG :: gen_heapGS Register Word Σ;
+  fst_llG :: traceG (list leak) Σ;
   fst_pcG :: traceG Word Σ;
   fst_progG :: traceG program Σ;
-  snd_traceG :: traceG (list leak) Σ;
+  snd_llG :: traceG (list leak) Σ;
   snd_pcG :: traceG Word Σ;
   snd_progG :: traceG program Σ;
 }.
 
+Definition binG1 `{binDG Σ} : asmGS Σ :=
+  {|
+    asmGS_invGS := bin_invG;
+    asm_memGS := fst_memG;
+    asm_regGS := fst_regG;
+    asm_llGS := fst_llG;
+    asm_pcGS := fst_pcG;
+    asm_progGS := fst_progG
+  |}.
+
+Definition binG2 `{binDG Σ} : asmGS Σ :=
+  {|
+    asmGS_invGS := bin_invG;
+    asm_memGS := snd_memG;
+    asm_regGS := snd_regG;
+    asm_llGS := snd_llG;
+    asm_pcGS := snd_pcG;
+    asm_progGS := snd_progG
+  |}.
+
+Definition prog1_frag `{!binDG Σ} := @tr_frag program Σ fst_progG.
+Definition pc1_frag `{!binDG Σ} := @tr_frag Word Σ fst_pcG.
+Definition ll1_frag `{!binDG Σ} := @tr_frag (list leak) Σ fst_llG.
+
+Definition prog2_frag `{!binDG Σ} := @tr_frag program Σ snd_progG.
+Definition pc2_frag `{!binDG Σ} := @tr_frag Word Σ snd_pcG.
+Definition ll2_frag `{!binDG Σ} := @tr_frag (list leak) Σ snd_llG.
+
+Definition prog1_auth `{!binDG Σ} := @tr_auth program Σ fst_progG.
+Definition pc1_auth `{!binDG Σ} := @tr_auth Word Σ fst_pcG.
+Definition ll1_auth `{!binDG Σ} := @tr_auth (list leak) Σ fst_llG.
+
+Definition prog2_auth `{!binDG Σ} := @tr_auth program Σ snd_progG.
+Definition pc2_auth `{!binDG Σ} := @tr_auth Word Σ snd_pcG.
+Definition ll2_auth `{!binDG Σ} := @tr_auth (list leak) Σ snd_llG.
+
 (* invariants for memory, and a state interpretation for (mem,reg) *)
-Global Instance irisG1 `{!binDG Σ} : irisGS asm_lang Σ := {
-    iris_invGS := bin_invG;
-    state_interp σ _ κs _ :=
-      ((@gen_heap_interp _ _ _ _ _ fst_regG (reg σ.1.2)) ∗
-         (@gen_heap_interp _ _ _ _ _ fst_memG (mem σ.1.2)) ∗
-         @tr_auth _ _ fst_traceG σ.2 ∗
-         @tr_auth _ _ fst_pcG (PC σ.1.2) ∗
-         @tr_auth _ _ fst_progG σ.1.1)%I;
-    fork_post _ := False%I;
-    num_laters_per_step _ := 0;
-    state_interp_mono _ _ _ _ := fupd_intro _ _
-  }.
+Print asm_irisGS.
+Global Instance irisG1 `{!binDG Σ} : irisGS asm_lang Σ := @asm_irisGS Σ binG1.
 
-Global Instance irisG2 `{!binDG Σ} : irisGS asm_lang Σ := {
-    iris_invGS := bin_invG;
-    state_interp σ _ κs _ :=
-      ((@gen_heap_interp _ _ _ _ _ snd_regG (reg σ.1.2)) ∗
-         (@gen_heap_interp _ _ _ _ _ snd_memG (mem σ.1.2)) ∗
-         @tr_auth _ _ snd_traceG σ.2 ∗
-         @tr_auth _ _ snd_pcG (PC σ.1.2) ∗
-         @tr_auth _ _ snd_progG σ.1.1)%I;
-    fork_post _ := False%I;
-    num_laters_per_step _ := 0;
-    state_interp_mono _ _ _ _ := fupd_intro _ _
-  }.
+Global Instance irisG2 `{!binDG Σ} : irisGS asm_lang Σ := @asm_irisGS Σ binG2.
 
-Definition TWP1 `{!binDG Σ} (e : expr) (E : coPset) (R : val → iProp Σ) :=
-  @twp (iProp Σ) expr val stuckness
+
+Definition TWP1 `{!binDG Σ} (e : AsmGen.expr) (E : coPset) (R : AsmGen.val → iProp Σ) :=
+  @twp (iProp Σ) AsmGen.expr AsmGen.val stuckness
     (@twp' _ asm_lang Σ irisG1)
     NotStuck E e R.
 
-Definition TWP2 `{!binDG Σ} (e : expr) (E : coPset) (R : val → iProp Σ) :=
-  @twp (iProp Σ) expr val stuckness
+Definition TWP2 `{!binDG Σ} (e : AsmGen.expr) (E : coPset) (R : AsmGen.val → iProp Σ) :=
+  @twp (iProp Σ) AsmGen.expr AsmGen.val stuckness
     (@twp' _ asm_lang Σ irisG2)
     NotStuck E e R.
 
-Section asm_lang_rules.
-  Context `{!binDG Σ}.
-  Context (γ ζ ξ : gname).
 (* Points to predicates for registers *)
-
 Definition pointsto_mem1 `{!binDG Σ} (a : Addr) (q : Qp) (w : Word) :=
     @pointsto Addr _ _ _ Σ fst_memG a (DfracOwn q) w.
 Definition pointsto_mem2 `{!binDG Σ} (a : Addr) (q : Qp) (w : Word) :=
@@ -108,37 +120,200 @@ Notation "r ↦2ₐ{ q } -" := (∃ w, r ↦2ₐ{q} w)%I
                              (at level 20, q at level 50, format "r  ↦2ₐ{ q }  -") : bi_scope.
 Notation "l ↦2ₐ -" := (l ↦2ₐ{1} -)%I (at level 20) : bi_scope.
 
-Lemma wp_halt pc prog ll E Φ :
-    prog pc = Halt ->
-    program1_frag program1_name prog -∗ pc1_frag pc1_name pc -∗ tr1_frag trace1_name ll -∗
-    program2_frag program2_name prog -∗ pc2_frag pc2_name pc -∗ tr2_frag trace2_name ll -∗
-    ▷ (program1_frag program1_name prog ∗ pc1_frag pc1_name pc ∗ tr1_frag trace1_name (NoLeak :: ll) -∗
-       program2_frag program2_name prog ∗ pc2_frag pc2_name pc ∗ tr2_frag trace2_name (NoLeak :: ll) -∗
-      Φ HaltedV) -∗
-    WP (Instr Executable, Instr Executable) @ E {{ v, Φ v }}.
+
+#[global] Instance binDG_irisDG `{!binDG Σ} : irisDG asm_lang Σ := {
+    state_rel := (λ σ1 σ2 κs1 κs2,
+                   @gen_heap_interp _ _ _ _ _ fst_regG (reg σ1.1.2) ∗
+                   @gen_heap_interp _ _ _ _ _ fst_memG (mem σ1.1.2) ∗
+                   @tr_auth _ _ fst_llG σ1.2 ∗
+                   @tr_auth _ _ fst_pcG (PC σ1.1.2) ∗
+                   @tr_auth _ _ fst_progG σ1.1.1 ∗
+                   @gen_heap_interp _ _ _ _ _ snd_regG (reg σ2.1.2) ∗
+                   @gen_heap_interp _ _ _ _ _ snd_memG (mem σ2.1.2) ∗
+                   @tr_auth _ _ snd_llG σ2.2 ∗
+                   @tr_auth _ _ snd_pcG (PC σ2.1.2) ∗
+                   @tr_auth _ _ snd_progG σ2.1.1
+  )%I
+  }.
+
+Section lifting.
+  Context `{!binDG Σ}.
+
+  Local Hint Extern 0 (base_reducible _ _) => eexists _, _, _; simpl : core.
+
+Lemma dwp_atomic_lift_wp Ψ1 Ψ2 E2 e1 e2 Φ
+  `{!Atomic StronglyAtomic e1}
+  `{!Atomic StronglyAtomic e2}
+  {NF1 : NoFork e1}
+  {NF2 : NoFork e2}
+  {He1 : NotVal e1}
+  {He2 : NotVal e2}:
+  TWP1 e1 E2 Ψ1 -∗
+  TWP2 e2 ∅ Ψ2 -∗
+  (∀ v1 v2, Ψ1 v1 -∗ Ψ2 v2 -∗ ▷ Φ v1 v2) -∗
+  dwp E2 e1 e2 Φ.
+Proof.
+  iIntros "HTWP1 HTWP2 H".
+  rewrite dwp_unfold /dwp_pre /= He1 He2.
+  iIntros (σ1 σ2 κ1 κs1 κ2 κs2) "Hσ".
+  iDestruct "Hσ" as "(Hregσ1 & Hmemσ1 & Hllσ1 & Hpcσ1 & Hprogσ1 &
+                      Hregσ2 & Hmemσ2 & Hllσ2 & Hpcσ2 & Hprogσ2)".
+  rewrite /TWP1 /TWP2 !twp_unfold /twp_pre /= !He1 !He2.
+  iSpecialize ("HTWP1" $! σ1 0 (κ1++κs1) 0 with "[$Hregσ1 $Hmemσ1 $Hllσ1 $Hpcσ1 $Hprogσ1]").
+  iSpecialize ("HTWP2" $! σ2 0 (κ2++κs2) 0%nat with "[$Hregσ2 $Hmemσ2 $Hllσ2 $Hpcσ2 $Hprogσ2]").
+  iMod "HTWP1" as (Hred1) "HTWP1".
+  iMod "HTWP2" as (Hred2) "HTWP2".
+  destruct Hred1 as (? & ? & ? & Hred1).
+  destruct Hred2 as (? & ? & ? & Hred2).
+  iModIntro.
+  iSplit. { iPureIntro. eexists. eauto. }
+  iSplit. { iPureIntro. eexists. eauto. }
+  iIntros (e1' σ1' efs e2' σ2' efs2 Hstep1 Hstep2).
+  iSpecialize ("HTWP1" $! [] e1' σ1' efs with "[//]").
+  iSpecialize ("HTWP2" with "[//]").
+  iMod "HTWP2" as "(_ & (Hreg2 & Hmem2 & Hll2 & Hpc2 & Hprog2) & HTWP2 & _)".
+  iMod "HTWP1" as "(_ & (Hreg1 & Hmem1 & Hll1 & Hpc1 & Hprog1) & HTWP1 & _)".
+  destruct (to_val e1') as [v1|] eqn:Hv1; last first.
+  { exfalso. destruct (atomic _ _ _ _ _ Hstep1). naive_solver. }
+  destruct (to_val e2') as [v2|] eqn:Hv2; last first.
+  { exfalso. destruct (atomic _ _ _ _ _ Hstep2). naive_solver. }
+  rewrite -(of_to_val _ _ Hv1) -(of_to_val _ _ Hv2).
+  rewrite !twp_value_fupd. iMod "HTWP1".
+  rewrite (fupd_mask_mono ∅ E2); last by set_solver.
+  iMod "HTWP2".
+  iFrame "Hreg2 Hmem2 Hll2 Hpc2 Hprog2
+    Hreg1 Hmem1 Hll1 Hpc1 Hprog1".
+  iApply step_fupd_intro; first set_solver.
+  iSpecialize ("H" with "HTWP1 HTWP2").
+  iNext. rewrite -dwp_value. iFrame "H".
+  rewrite (nofork _ _ _ _ _ Hstep1).
+  rewrite (nofork _ _ _ _ _ Hstep2).
+  simpl. eauto with iFrame.
+Qed.
+
+
+Lemma dwp_halt (pc1 pc2 : Word) (prog1 prog2 : program) (ll1 ll2 : list leak) E Φ :
+    prog1 pc1 = Halt ->
+    prog2 pc2 = Halt ->
+    prog1_frag prog1 -∗ pc1_frag pc1 -∗ ll1_frag ll1 -∗
+    prog2_frag prog2 -∗ pc2_frag pc2 -∗ ll2_frag ll2 -∗
+    ▷ (prog1_frag prog1 ∗ pc1_frag pc1 ∗ ll1_frag (NoLeak :: ll1) -∗
+       prog2_frag prog2 ∗ pc2_frag pc2 ∗ ll2_frag (NoLeak :: ll2) -∗
+      Φ HaltedV HaltedV) -∗
+    dwp E (Instr Executable) (Instr Executable) Φ.
   Proof.
-    iIntros (prpcHalt) "Hprog Hpc Hll HΦ".
-    iApply wp_lift_atomic_step_no_fork_fupd; auto.
-    iIntros (σ ns κ κs nt) "(Hauthreg & Hauthmem & Hauthtrace & Hauthpc & Hauthprog)".
-    destruct σ as [s ll'].
-    simpl.
-    iDestruct (@trace_full_frag_eq with "Hauthtrace Hll") as %?; subst; auto.
-    iDestruct (@pc_full_frag_eq with "Hauthpc Hpc") as %?; subst; auto.
-    iDestruct (@program_full_frag_eq with "Hauthprog Hprog") as %?; subst; auto.
-    iModIntro.
-    iSplitR.
-    - iPureIntro. apply normal_always_reducible.
-    - iIntros (e2 σ2 efs) "%steps test".
-      inversion steps; subst; simpl in *.
-      inversion H; subst.
-      simpl in *.
-      rewrite prpcHalt in steps. rewrite prpcHalt. simpl in *. iFrame.
-      iPoseProof (trace_update trace_name _ (NoLeak :: ll) with "[$Hauthtrace $Hll]") as "H".
-      iMod "H". iModIntro. iNext. iModIntro.
-      iDestruct "H" as "[Hauthll Hfragll]". iFrame.
-      iSplitR.
-      { iPureIntro; reflexivity. }
-      iApply "HΦ". iFrame.
+    iIntros (prpc1Halt prpc2Halt) "Hprog1 Hpc1 Hll1 Hprog2 Hpc2 Hll2 HΦ".
+    iApply (dwp_atomic_lift_wp
+              (λ v, ⌜v = HaltedV⌝ ∗ prog1_frag prog1 ∗ pc1_frag pc1 ∗ ll1_frag (NoLeak :: ll1))%I
+              (λ v, ⌜v = HaltedV⌝ ∗ prog2_frag prog2 ∗ pc2_frag pc2 ∗ ll2_frag (NoLeak :: ll2))%I
+             with "[Hprog1 Hpc1 Hll1] [Hprog2 Hpc2 Hll2] [HΦ]").
+    { iApply (twp_halt with "[Hprog1] [Hpc1] [Hll1] []"); try iFrame; eauto. }
+    { iApply (twp_halt with "[Hprog2] [Hpc2] [Hll2] []"); eauto. }
+    iIntros (? ?) "(% & Hprog1 & Hpc1 & Hll1) (% & Hprog2 & Hpc2 & Hll2)". subst.
+    iNext.
+    iApply ("HΦ" with "[$Hprog1 $Hpc1 $Hll1] [$Hprog2 $Hpc2 $Hll2]").
   Qed.
 
+  Definition dwp_bind_loop_executable
+    (E : coPset)
+    (Φ : language.val asm_lang → language.val asm_lang → iProp Σ) :
+    dwp E (Instr Executable) (Instr Executable)
+      (fun v1 v2 => (dwp E (loopify (language.of_val v1)) (loopify (language.of_val v2)) Φ))
+   ⊢ dwp E (loopify (Instr Executable)) (loopify (Instr Executable)) Φ :=
+   dwp_bind loopify loopify E (Instr Executable) (Instr Executable) Φ.
 
+
+Lemma dwp_loop_next Φ E :
+  dwp E (Loop Executable) (Loop Executable) Φ ⊢
+  dwp E (Loop NextI) (Loop NextI) Φ.
+  Proof.
+    iIntros "HExec".
+    iApply dwp_lift_pure_step_no_fork; auto;
+    try apply loop_next_always_reducible.
+    { intros κ σ1 e2 σ1' efs steps. inversion steps. auto. }
+    { intros κ σ2 e2 σ2' efs steps. inversion steps. auto. }
+    
+    iModIntro. iNext. iModIntro.
+    
+    iIntros (κ1 κ2 e1' σ1 efs1 e2' σ2 efs2) "%steps1 %steps2".
+    inversion steps1; inversion steps2; auto.
+Qed.
+
+Lemma dwp_loop_halted Φ E :
+  Φ LoopHaltedV LoopHaltedV -∗
+  dwp E (Loop Halted) (Loop Halted) Φ.
+  Proof.
+    iIntros "HΦ".
+    iApply (dwp_value _ _ _ _ LoopHaltedV LoopHaltedV); try reflexivity; try auto.
+Qed.
+
+  Lemma test_prog_not_constant_time_different_leakage Φ :
+  prog1_frag (test_prog_not_constant_time 2) -∗
+  prog2_frag (test_prog_not_constant_time 0) -∗
+  pc1_frag (word 0) -∗ pc2_frag (word 0) -∗
+  ll1_frag [] -∗ ll2_frag [] -∗
+  register 0 ↦1ᵣ word 0 -∗
+  register 0 ↦2ᵣ word 0 -∗
+  ▷(∀ ll ll', prog1_frag (test_prog_not_constant_time 2) -∗
+    prog2_frag (test_prog_not_constant_time 0) -∗
+    pc1_frag (word 3) -∗ pc2_frag (word 2) -∗
+    ll1_frag ll -∗ ll2_frag ll' -∗
+    ⌜ll ≠ ll'⌝ -∗
+      Φ LoopHaltedV LoopHaltedV) -∗
+    dwp ∅ (Loop Executable) (Loop Executable) Φ.
+  Proof.
+    iIntros "Hprog1 Hprog2 Hpc1 Hpc2 Hll1 Hll2 Hr1 Hr2 HΦ".
+    iApply dwp_bind_loop_executable.
+    iApply (dwp_atomic_lift_wp
+              (λ v, ⌜v = NextIV⌝ ∗ prog1_frag (test_prog_not_constant_time 2) ∗ pc1_frag (word 1) ∗ ll1_frag [NoLeak] ∗ [∗ map] k↦y ∈ <[register 0:=add_vec_2 (inputs_from_inputnatregs (<[register 0:=word 0]> ∅) [#inl (word 2); inl (word 2)])]> (<[register 0:=word 0]> ∅), k ↦1ᵣ y )%I
+              (λ v, ⌜v = NextIV⌝ ∗ prog2_frag (test_prog_not_constant_time 0) ∗ pc2_frag (word 1) ∗ ll2_frag [NoLeak] ∗ [∗ map] k↦y ∈ <[register 0:=add_vec_2 [#word 0; word 0]]> (<[register 0:=word 0]> ∅), k ↦2ᵣ y)%I
+             with "[Hprog1 Hpc1 Hll1 Hr1] [Hprog2 Hpc2 Hll2 Hr2] [HΦ]").
+    { iApply (twp_computation (<[register 0 := word 0]> empty)
+               with "[Hprog1] [Hpc1] [Hll1] [Hr1]"); try iFrame; try reflexivity.
+      { econstructor; try reflexivity. }
+      { iApply big_sepM_insert. { constructor. }
+        iFrame. by iApply big_sepM_empty. }
+      iIntros "(Hprog & Hpc & Hll & H)". simpl. iFrame. iPureIntro. reflexivity. }
+    { iApply (twp_computation (<[register 0 := word 0]> empty)
+               with "[Hprog2] [Hpc2] [Hll2] [Hr2]"); try iFrame; try reflexivity.
+      { econstructor; try reflexivity. }
+      { iApply big_sepM_insert. { constructor. }
+        iFrame. by iApply big_sepM_empty. }
+      iIntros "(Hprog & Hpc & Hll & H)". simpl. iFrame. iPureIntro. reflexivity. }
+
+     iIntros (? ?) "(-> & Hprog1 & Hpc1 & Hll1 & Hr1) (-> & Hprog2 & Hpc2 & Hll2 & Hr2)".
+     simpl. iNext.    
+     iApply dwp_loop_next.
+
+     iApply dwp_bind_loop_executable.
+     iApply (dwp_atomic_lift_wp
+               (λ v, ⌜v = NextIV⌝ ∗ prog1_frag (test_prog_not_constant_time 2) ∗ pc1_frag (word 3) ∗ ll1_frag [ControlFlowLeak (notzero_vec_1 [#<[register 0:=word 4]> ∅ !!! register 0]); NoLeak] ∗ [∗ map] k↦y ∈ <[register 0:=word 4]> ∅, k ↦1ᵣ y)%I
+               (λ v, ⌜v = NextIV⌝ ∗ prog2_frag (test_prog_not_constant_time 0) ∗ pc2_frag (word 2) ∗ ll2_frag [ControlFlowLeak (notzero_vec_1 [#<[register 0:=word 0]> ∅ !!! register 0]); NoLeak] ∗ [∗ map] k↦y ∈ <[register 0:=word 0]> ∅, k ↦2ᵣ y)%I
+              with "[Hprog1 Hpc1 Hll1 Hr1] [Hprog2 Hpc2 Hll2 Hr2] [HΦ]").
+     { iApply (twp_control_flow (<[register 0:= word 4]> ∅) with "[Hprog1] [Hpc1] [Hll1] [Hr1]"); try iFrame; try reflexivity.
+       { econstructor; reflexivity. }
+       iIntros "(Hprog & Hpc & Hll & Hmap)".
+       simpl. iFrame. iPureIntro. reflexivity.
+     }
+     { iApply (twp_control_flow (<[register 0:= word 0]> ∅) with "[Hprog2] [Hpc2] [Hll2] [Hr2]"); try iFrame; try reflexivity.
+       { econstructor; reflexivity. }
+       iIntros "(Hprog & Hpc & Hll & Hmap)".
+       simpl. iFrame. iPureIntro. reflexivity.
+     }
+
+
+     iIntros (? ?) "(-> & Hprog1 & Hpc1 & Hll1 & Hr1) (-> & Hprog2 & Hpc2 & Hll2 & Hr2)".
+     simpl. iNext.    
+     iApply dwp_loop_next.
+     iApply dwp_bind_loop_executable.
+     iApply (dwp_halt with "Hprog1 Hpc1 Hll1 Hprog2 Hpc2 Hll2"); try reflexivity.
+     iNext. iIntros "(Hprog1 & Hpc1 & Hll1) (Hprog2 & Hpc2 & Hll2)".
+     iApply dwp_loop_halted. iApply ("HΦ" with "Hprog1 Hprog2 Hpc1 Hpc2 Hll1 Hll2").
+     iPureIntro.
+     intro H.
+
+     apply (f_equal (fun l => nth 1 l NoLeak)) in H. simpl in H.
+     do 2 (rewrite lookup_total_insert in H).
+     unfold notzero_vec_1 in H. unfold unaryOn1Vec in H. simpl in H.
+     congruence.
+Qed.
